theories/TransVal/CombineEnv.v
@@ -10,334 +10,73 @@ Definition combineEnv D (E1:onv val) E2 :=
 
 (** Lemmata **)
 
-Lemma combineenv_agree D E E'
+Lemma combineEnv_agree D E E'
   : agree_on eq D (combineEnv D E E') E.
 Proof.
   hnf; intros. unfold combineEnv. cases; eauto; isabsurd.
 Qed.
 
-Lemma exp_combineenv_eql e D Es Et v
-  : Exp.freeVars e ⊆ D
-    -> (exp_eval (combineEnv D Es Et) e = v <-> exp_eval Es e = v).
+Lemma combineEnv_agree_meet D D' Es Et
+  : agree_on eq (D' ∩ D) Es Et
+    -> agree_on eq D' (combineEnv D Es Et) Et.
 Proof.
-  intros. split; intros.
-  - eapply (exp_eval_agree (E:=(combineEnv D Es Et))); eauto.
-    eapply (agree_on_incl (bv:= Exp.freeVars e) (lv:= D));
-      cset_tac; eauto.
-    eapply combineenv_agree.
-  - eapply (exp_eval_agree (E:=Es)); eauto.
-    eapply (agree_on_incl (bv:=Exp.freeVars e) (lv:=D)); eauto.
-    symmetry. eapply combineenv_agree.
+ intros.
+ - hnf. cset_tac. unfold combineEnv. cases; eauto.
+   rewrite H; eauto. cset_tac; intuition.
 Qed.
 
-Lemma explist_combineenv_eql el D Es Et rl
-  : list_union (List.map Exp.freeVars el) ⊆ D
-    -> ( omap (exp_eval (combineEnv D Es Et)) el = rl <-> omap (exp_eval Es) el = rl).
+Lemma combineEnv_agree_minus D D' Es Et
+  : agree_on eq (D' \ D) Es Et
+    -> agree_on eq D' (combineEnv D Es Et) Es.
 Proof.
-  intros.
-  general induction el; simpl in * |- *; eauto.
-  - reflexivity.
-  - rewrite list_union_start_swap in H.
-    pose proof (exp_combineenv_eql a D Es Et (exp_eval (combineEnv D Es Et) a));
-      eauto.
-      destruct H0; [ hnf; intros; eauto with cset | ].
-    * rewrite H0; eauto.
-      edestruct (IHel D Es Et); [ hnf; intros; eauto with cset| ].
-      erewrite H3; eauto. reflexivity.
+ intros.
+ - hnf. cset_tac. unfold combineEnv. cases; eauto.
+   rewrite H; eauto. cset_tac; intuition.
 Qed.
 
-Lemma combineenv_eql:
-forall F s D Es Et,
- freeVars s ⊆  D
-->(  models F (to_total Es) s  <-> models F (to_total (combineEnv D Es Et)) s).
-
+Lemma combineEnv_models F s D Es Et
+  : freeVars s ⊆  D
+    -> (models F (to_total Es) s  <-> models F (to_total (combineEnv D Es Et)) s).
 Proof.
   intros. eapply models_agree. eapply (agree_on_incl (lv:=D)); eauto; symmetry.
   eapply agree_on_total.
-  eapply combineenv_agree.
+  eapply combineEnv_agree.
 Qed.
 
-Lemma exp_combineenv_eqr:
-forall e D Es Et v,
-agree_on eq (Exp.freeVars e ∩ D) Es Et
--> (exp_eval (combineEnv D Es Et) e= v <-> exp_eval Et e = v).
-
+Lemma combineEnv_omap_exp_eval_left el D Es Et
+  : list_union (List.map Exp.freeVars el) ⊆ D
+    -> omap (exp_eval (combineEnv D Es Et)) el = omap (exp_eval Es) el.
 Proof.
- intros; split; intros.
- - eapply (exp_eval_agree (E:=(combineEnv D Es Et))); eauto.
-   hnf. cset_tac. unfold combineEnv. cases; eauto.
-   eapply H. cset_tac; intuition.
- - eapply (exp_eval_agree (E:= Et)); eauto.
-   hnf; cset_tac. unfold combineEnv; cases; eauto.
-   symmetry. eapply H; cset_tac; intuition.
+  intros.
+  erewrite omap_exp_eval_agree; [reflexivity | | reflexivity].
+  symmetry. eapply agree_on_incl; eauto using combineEnv_agree.
 Qed.
 
-Lemma exp_combineenv_eqr':
-forall e D Es Et v,
-agree_on eq (Exp.freeVars e ∩ D) Es Et
--> (exp_eval (to_partial (to_total (combineEnv D Es Et))) e
-   = v <-> exp_eval (to_partial (to_total Et)) e = v).
-
+Lemma combineEnv_omap_exp_eval_right el D Es Et
+  : agree_on eq (list_union (List.map Exp.freeVars el) ∩ D) Es Et
+    -> omap (exp_eval (combineEnv D Es Et)) el = omap (exp_eval Et) el.
 Proof.
- intros; split; intros.
- - eapply (exp_eval_agree (E:=(to_partial (to_total (combineEnv D Es Et))))); eauto.
-   hnf. cset_tac. unfold combineEnv, to_partial, to_total. cases; eauto.
-   rewrite H. reflexivity. cset_tac; intuition.
- - eapply (exp_eval_agree (E:= to_partial (to_total Et))); eauto.
-   hnf; cset_tac. unfold combineEnv, to_partial, to_total; cases; eauto.
-   rewrite H. reflexivity.
-   cset_tac; intuition.
+  intros.
+  erewrite omap_exp_eval_agree; [reflexivity | | reflexivity].
+  symmetry. eapply combineEnv_agree_meet; eauto.
 Qed.
 
-Lemma explist_combineenv_eqr:
-forall el D Es Et vl,
-agree_on eq (list_union (List.map Exp.freeVars el) ∩ D) Es Et
--> (omap (exp_eval (combineEnv D Es Et)) el = vl <-> omap (exp_eval Et) el = vl).
-
-Proof.
-  intros; split; intros.
-  - general induction el.
-    + reflexivity.
-    + simpl in *; hnf in H.
-      pose proof (exp_combineenv_eqr a D Es Et (exp_eval (combineEnv D Es Et) a)).
-      destruct H0.
-      * hnf; intros; cset_tac. eapply H. split; eauto.
-        eapply list_union_start_swap; cset_tac; eauto.
-      * rewrite H0; eauto. f_equal.
-        rewrite (IHel D Es Et (omap (exp_eval (combineEnv D Es Et)) el)); eauto.
-        hnf. intros. cset_tac. eapply H. split; eauto.
-        eapply list_union_start_swap. cset_tac; eauto.
-  - general induction el.
-    + reflexivity.
-    + simpl in *; hnf in H.
-      pose proof (exp_combineenv_eqr a D Es Et (exp_eval Et a)).
-      destruct H0.
-      * hnf; intros; cset_tac. eapply H. split; eauto.
-        eapply list_union_start_swap; cset_tac; eauto.
-      * rewrite H1; eauto. f_equal.
-        symmetry. rewrite (IHel D Es Et (omap (exp_eval  Et) el)); eauto.
-        hnf. intros. cset_tac. eapply H. split; eauto.
-        eapply list_union_start_swap. cset_tac; eauto.
-Qed.
-
-Lemma explist_combineenv_eqr':
-forall el D Es Et vl,
-  agree_on eq (list_union (List.map Exp.freeVars el) ∩ D) Es Et
-  -> (omap (exp_eval (to_partial (to_total (combineEnv D Es Et)))) el = vl
-                     <-> omap (exp_eval (to_partial (to_total Et))) el = vl).
-
-Proof.
-  intros; split; intros.
-  - general induction el.
-    +  reflexivity.
-    + simpl in *; hnf in H.
-      pose proof (exp_combineenv_eqr' a D Es Et (exp_eval (to_partial (to_total (combineEnv D Es Et))) a)).
-      destruct H0.
-      * hnf; intros; cset_tac. eapply H; split; eauto.
-        eapply list_union_start_swap; cset_tac; eauto.
-      * rewrite H0; eauto. f_equal.
-        symmetry. simpl.
-        rewrite (IHel D Es Et (omap (exp_eval (to_partial (to_total (combineEnv D Es Et)))) el)); eauto.
-        hnf; intros; cset_tac. eapply H; split; eauto.
-        eapply list_union_start_swap. cset_tac; eauto.
-  - general induction el.
-    + reflexivity.
-    + simpl in *; hnf in H.
-      pose proof (exp_combineenv_eqr' a D Es Et (exp_eval (to_partial (to_total Et)) a)).
-      destruct H0.
-      * hnf; intros; cset_tac. eapply H; split; eauto.
-        eapply list_union_start_swap; cset_tac; eauto.
-      * rewrite H1; eauto. f_equal.
-        symmetry. simpl.
-        rewrite (IHel D Es Et (omap (exp_eval (to_partial (to_total Et))) el)); eauto.
-        hnf; intros; cset_tac. eapply H; split; eauto.
-        eapply list_union_start_swap. cset_tac; eauto.
-Qed.
-
-Lemma combineenv_eqr:
-  forall  F s D Es Et,
-    agree_on eq (freeVars s ∩ D) Es Et
-    -> (models F (to_total Et) s <-> models F (to_total (combineEnv D Es Et)) s).
-
-Proof.
-  intros.  general induction s; try reflexivity; simpl in * |- *.
-  - rewrite (IHs1 F D Es Et); eauto with cset.
-    rewrite (IHs2 F D Es Et); eauto with cset.
-    reflexivity.
-  - rewrite (IHs1 F D Es Et); eauto with cset.
-    rewrite (IHs2 F D Es Et); eauto with cset.
-    reflexivity.
-  - rewrite (IHs F D Es Et); eauto with cset.
-    reflexivity.
-  - case_eq (exp_eval (to_partial (to_total (combineEnv D Es Et))) e); intros.
-    + pose proof (exp_combineenv_eqr' e D Es Et (Some v)).
-      assert (agree_on eq (Exp.freeVars e ∩ D) Es Et).
-      * hnf; intros. hnf in H. simpl in H. cset_tac.
-      * destruct H1; eauto.
-        specialize (H1 H0).
-        unfold smt_eval; rewrite H1.
-        case_eq (val2bool v); intros.
-        { rewrite (IHs1 F D Es Et); eauto with cset.
-          rewrite H0, H4. reflexivity.
-        }
-        { rewrite (IHs2 F D Es Et); eauto with cset.
-          rewrite H0, H4. reflexivity.
-        }
-     + pose proof (exp_combineenv_eqr' e D Es Et None).
-       assert (agree_on eq (Exp.freeVars e ∩ D) Es Et).
-       * hnf; intros. hnf in H. simpl in H. cset_tac.
-       * destruct H1; eauto.  specialize (H1 H0).
-         unfold smt_eval; rewrite H0, H1.
-         case_eq (val2bool undef_substitute); intros.
-         { rewrite (IHs1 F D Es Et); eauto with cset.
-           reflexivity. }
-         { rewrite (IHs2 F D Es Et); eauto with cset.
-           reflexivity. }
-  - rewrite (IHs1 F D Es Et); eauto with cset.
-    rewrite (IHs2 F D Es Et); eauto with cset.
-    reflexivity.
-  - case_eq (exp_eval (to_partial (to_total (combineEnv D Es Et))) e); intros;
-    case_eq (exp_eval (to_partial (to_total (combineEnv D Es Et))) e0); intros.
-    + pose proof (exp_combineenv_eqr' e D Es Et (Some v)).
-       assert (agree_on eq (Exp.freeVars e ∩ D) Es Et).
-       * hnf; intros. hnf in H. simpl in H. cset_tac.
-       * destruct H2; eauto. specialize (H2 H0).
-         pose proof (exp_combineenv_eqr' e0 D Es Et (Some v0)).
-         assert (agree_on eq (Exp.freeVars e0 ∩ D) Es Et).
-       { hnf; intros. hnf in H. simpl in H. cset_tac. }
-       { destruct H5; eauto. specialize (H5 H1).
-         unfold smt_eval.
-         rewrite H2, H5, H4, H7; eauto; intuition.
-       }
-    + pose proof (exp_combineenv_eqr' e D Es Et (Some v)).
-      assert (agree_on eq (Exp.freeVars e ∩ D) Es Et) by eauto with cset.
-      destruct H2; eauto. specialize (H2 H0).
-      pose proof (exp_combineenv_eqr' e0 D Es Et None).
-      assert (agree_on eq (Exp.freeVars e0 ∩ D) Es Et) by eauto with cset.
-      destruct H5; eauto. specialize (H5 H1).
-      unfold smt_eval.
-      rewrite H0, H1, H2, H5; intuition.
-    + pose proof (exp_combineenv_eqr' e D Es Et None).
-      assert (agree_on eq (Exp.freeVars e ∩ D) Es Et) by eauto with cset.
-      destruct H2; eauto. specialize (H2 H0).
-      pose proof (exp_combineenv_eqr' e0 D Es Et (Some v)).
-      destruct H5; eauto with cset.
-      { specialize (H5 H1).
-        unfold smt_eval.
-        rewrite H0, H1, H2, H5.
-        intuition. }
-    + pose proof (exp_combineenv_eqr' e D Es Et None).
-      assert (agree_on eq (Exp.freeVars e ∩ D) Es Et) by eauto with cset.
-      destruct H2; eauto. specialize (H2 H0).
-      pose proof (exp_combineenv_eqr' e0 D Es Et None).
-      destruct H5; eauto with cset.
-      { unfold smt_eval. rewrite H0, H1, H2, H5; eauto.
-        intuition. }
-  -  simpl. unfold labInc. destruct p.
-     (* TODO: Make Lemma *)
-     assert ((List.map (smt_eval (to_total Et)) a)
-     = (List.map (smt_eval (to_total (combineEnv D Es Et))) a)).
-     + general induction a.
-       * eauto.
-       * simpl.
-         pose proof (exp_combineenv_eqr' a D Es Et (exp_eval (to_partial (to_total Et)) a)).
-         pose proof (exp_combineenv_eqr' a D Es Et
-                                         (exp_eval (to_partial (to_total (combineEnv D Es Et))) a)).
-         simpl in *. rewrite list_union_start_swap in H.
-         destruct H0; eauto with cset.
-         { destruct H1; eauto with cset.
-           - clear H3. clear H0.
-             unfold smt_eval at 1. rewrite H1; eauto.
-             unfold smt_eval at 2.
-             destruct (exp_eval (to_partial (to_total (combineEnv D Es Et))) a);
-               f_equal.
-             + erewrite (IHa n _ D Es Et); eauto with cset.
-             + erewrite (IHa n _ D Es Et); eauto with cset.
-         }
-     + rewrite H0; intuition.
-    Grab Existential Variables.
-    econstructor.
-    econstructor.
-Qed.
-
-Lemma renamed_apart_contained x e L E s Es D:
-  x \In Exp.freeVars e
-  -> Terminates (L, E, s) (L, Es, stmtReturn e)
+Lemma renamedApart_contained L E s t Es D
+: Terminates (L, E, s) (L, Es, t)
   -> noFun s
   -> renamedApart s D
-  -> x \In (fst(getAnn D)) \/ x \In (snd (getAnn D)).
+  -> IL.freeVars t ⊆ fst (getAnn D) ∪ snd (getAnn D).
 
 Proof.
-  intros fv_e term_s nf_s ssa_s.
-  general induction term_s.
-  - inv ssa_s.
-    cset_tac.
-  - inv H; inv ssa_s; inv nf_s; simpl.
-    + specialize (IHterm_s x e L' (E0 [x0 <- ⎣ v ⎦]) s' Es an fv_e).
-      destruct IHterm_s as [in_fv | in_dv]; auto.
-      * rewrite H8.
-        rewrite H9 in in_fv; simpl in in_fv.
-        cset_tac.
-      * rewrite H8.
-        rewrite H9 in in_dv; simpl in in_dv.
-        cset_tac.
-    + specialize (IHterm_s x e L' E' s' Es ans).
-      destruct IHterm_s as [in_fv | in_dv]; auto.
-      * rewrite <- H6.
-        rewrite H10 in in_fv; simpl in in_fv.
-        cset_tac.
-      * rewrite <- H6.
-        rewrite H10 in in_dv; simpl in in_dv.
-        cset_tac.
-    + specialize (IHterm_s x e L' E' s' Es ant).
-      destruct IHterm_s as [in_fv | in_dv]; auto.
-      * rewrite <- H6.
-        rewrite H11 in in_fv; simpl in in_fv.
-        cset_tac.
-      * rewrite <- H6.
-        rewrite H11 in in_dv; simpl in in_dv.
-        cset_tac.
-    + specialize (H0 l Y); isabsurd.
-Qed.
-
-Lemma renamed_apart_contained_list x X L E s Es f D:
-  x \In list_union (Exp.freeVars ⊝ X)
-  -> Terminates (L,E,s) (L, Es, stmtApp f X)
-  -> noFun s
-  -> renamedApart s D
-  -> x \In (fst (getAnn D)) \/ x \In (snd (getAnn D)).
-
-Proof.
-  intros fv_e term_s nf_s ssa_s.
-  general induction term_s.
-  - inv ssa_s.
-    cset_tac.
-  - inv H; inv ssa_s; inv nf_s; simpl.
-    + specialize (IHterm_s x X L' (E0 [x0 <- ⎣ v ⎦]) s' Es f an fv_e).
-      destruct IHterm_s as [in_fv | in_dv]; auto.
-      * rewrite H8.
-        rewrite H9 in in_fv; simpl in in_fv.
-        cset_tac.
-      * rewrite H8.
-        rewrite H9 in in_dv; simpl in in_dv.
-        cset_tac.
-    + specialize (IHterm_s x X L' E' s' Es f ans).
-      destruct IHterm_s as [in_fv | in_dv]; auto.
-      * rewrite <- H6.
-        rewrite H10 in in_fv; simpl in in_fv.
-        cset_tac.
-      * rewrite <- H6.
-        rewrite H10 in in_dv; simpl in in_dv.
-        cset_tac.
-    + specialize (IHterm_s x X L' E' s' Es f ant).
-      destruct IHterm_s as [in_fv | in_dv]; auto.
-      * rewrite <- H6.
-        rewrite H11 in in_fv; simpl in in_fv.
-        cset_tac.
-      * rewrite <- H6.
-        rewrite H11 in in_dv; simpl in in_dv.
-        cset_tac.
-    + specialize (H0 l Y); isabsurd.
+  intros term_s nf_s ssa_s.
+  general induction term_s; invt noFun; invt renamedApart; try invt F.step; simpl; eauto with cset.
+  - exploit IHterm_s as IH; try reflexivity; eauto.
+    rewrite IH. pe_rewrite. rewrite H9. clear_all; cset_tac.
+  - exploit IHterm_s as IH; try reflexivity; eauto.
+    rewrite IH. pe_rewrite. rewrite <- H8. clear_all; cset_tac.
+  - exploit IHterm_s as IH; try reflexivity; eauto.
+    rewrite IH. pe_rewrite. rewrite <- H8. clear_all; cset_tac.
+  - exfalso; eapply H0; eauto.
 Qed.
 
 Lemma agree_on_ssa_combine:
@@ -357,39 +96,21 @@ Proof.
   intros D D' L E s t Es Et es et.
   intros ssa_s ssa_t agree_fv disj_dv nf_s nf_t sterm tterm.
   split.
-  - pose proof (ssa_move_return D' L E t Et et nf_t ssa_t tterm).
-    destruct H as [D'' [ ssaRet [fstSubset sndSubset]]].
-    inv ssaRet.
-    hnf.
-    intros x fv_Et.
+  - edestruct (ssa_move_return D' L E t Et et nf_t ssa_t tterm)
+      as [D'' [ ssaRet [fstSubset sndSubset]]].
+    exploit term_ssa_eval_agree; try eapply sterm; eauto.
+    exploit term_ssa_eval_agree; try eapply tterm; eauto.
+    exploit (renamedApart_contained L E t (stmtReturn et) Et D') as fv_dv; eauto.
+    simpl in *. symmetry.
+    eapply agree_on_incl; [ eapply combineEnv_agree_meet | reflexivity ].
+    rewrite fv_dv. rewrite <- agree_fv.
+    rewrite <- agree_fv in H0. rewrite H in H0; clear H.
+    hnf; intros; cset_tac.
+  - edestruct (ssa_move_return D L E s Es es nf_s ssa_s sterm)
+      as [D'' [ssaRet [fstSubset sndSubset]]]; eauto.
+    inv ssaRet. symmetry.
+    eapply agree_on_incl; [eapply combineEnv_agree_minus | reflexivity ].
+    exploit (renamedApart_contained L E s (stmtReturn es) Es D) as fv_dv; eauto.
     simpl in *.
-    unfold combineEnv.
-    cases; try reflexivity.
-    + cset_tac.
-      * pose proof (term_ssa_eval_agree L L s D (stmtReturn es) E Es ssa_s nf_s sterm).
-        pose proof (term_ssa_eval_agree L L t D' (stmtReturn et) E Et ssa_t nf_t tterm).
-        hnf in H2, H3.
-        rewrite <- (H2 x H).
-        rewrite (agree_fv x) in H.
-        rewrite <- (H3 x H).
-        reflexivity.
-      * exfalso.
-        pose proof (renamed_apart_contained x et L E t Et D') as fv_dv.
-        destruct fv_dv as [in_fv | in_dv]; auto.
-        pose proof (renamedApart_disj ssa_s) as disj_fv_dv.
-        unfold disj in disj_fv_dv.
-        apply (disj_fv_dv x); auto.
-        rewrite (agree_fv x); auto.
-  - pose proof (ssa_move_return D L E s Es es nf_s ssa_s sterm).
-    destruct H as [D'' [ssaRet [fstSubset sndSubset]]].
-    inv ssaRet.
-    simpl in *.
-    hnf; intros.
-    unfold combineEnv.
-    cases; auto.
-    exfalso.
-    apply NOTCOND. hnf in H0. specialize (H0 x H).
-    cset_tac.
-    pose proof (renamed_apart_contained x es L E s Es D) as fv_dv.
-    destruct fv_dv; auto.
+    rewrite fv_dv. hnf; intros; cset_tac.
 Qed.
